Minterm.thy
@@ -15,73 +15,73 @@ subsection {* Minterms Definition *}
 
 typedef ('var, 'k::finite) minterm 
   = "{S. ((\<exists>!l\<in>S::('var, 'k::finite) literal set. \<exists>n. 
-          (to_sl_formula l) = (ext_card_heap_superior_to n))
+          (to_sl_formula l) = (ext_card_heap_ge n))
         \<and> (\<exists>!l\<in>S::('var, 'k::finite) literal set. \<exists>n. 
-          (to_sl_formula l) = (not (ext_card_heap_superior_to n))))}"
+          (to_sl_formula l) = (not (ext_card_heap_ge n))))}"
 proof
-  define l1::"('var, 'k::finite) sl_formula" where "l1 = ext_card_heap_superior_to 0"
+  define l1::"('var, 'k::finite) sl_formula" where "l1 = ext_card_heap_ge 0"
   have "l1\<in> test_formulae" unfolding l1_def using test_formulae.simps by auto
   define x::"('var, 'k::finite) literal set"
     where "x = {to_literal l1, to_literal (not l1)}"
   show "x \<in> {S. ((\<exists>!l\<in>S::('var, 'k::finite) literal set. \<exists>n. 
-            (to_sl_formula l) = (ext_card_heap_superior_to n))
+            (to_sl_formula l) = (ext_card_heap_ge n))
           \<and> (\<exists>!l\<in>S::('var, 'k::finite) literal set. \<exists>n. 
-            (to_sl_formula l) = (not (ext_card_heap_superior_to n))))}"
+            (to_sl_formula l) = (not (ext_card_heap_ge n))))}"
   proof (intro CollectI conjI ex1I)
     show "to_literal l1 \<in> x" by (simp add: l1_def x_def) 
-    show "\<exists>n. to_sl_formula (to_literal l1) = ext_card_heap_superior_to n"
+    show "\<exists>n. to_sl_formula (to_literal l1) = ext_card_heap_ge n"
     proof
-      show "to_sl_formula (to_literal l1) = ext_card_heap_superior_to 0" using \<open>l1\<in> test_formulae\<close>
+      show "to_sl_formula (to_literal l1) = ext_card_heap_ge 0" using \<open>l1\<in> test_formulae\<close>
         unfolding l1_def by simp     
     qed
-    show "\<And>l. l \<in> x \<and> (\<exists>n. to_sl_formula l = ext_card_heap_superior_to n) \<Longrightarrow> l = to_literal l1"
+    show "\<And>l. l \<in> x \<and> (\<exists>n. to_sl_formula l = ext_card_heap_ge n) \<Longrightarrow> l = to_literal l1"
     proof -
       fix l
-      assume lprop: "l \<in> x \<and> (\<exists>n. to_sl_formula l = ext_card_heap_superior_to n)"
-      hence "\<exists>n. to_sl_formula l = ext_card_heap_superior_to n" by simp
-      from this obtain n where ndef: "to_sl_formula l = ext_card_heap_superior_to n" by auto
+      assume lprop: "l \<in> x \<and> (\<exists>n. to_sl_formula l = ext_card_heap_ge n)"
+      hence "\<exists>n. to_sl_formula l = ext_card_heap_ge n" by simp
+      from this obtain n where ndef: "to_sl_formula l = ext_card_heap_ge n" by auto
       have "l = to_literal l1 \<or> l = to_literal (not l1)" using lprop unfolding x_def by simp
       moreover have "l\<noteq> to_literal (not l1)"
       proof (rule ccontr)
         assume "\<not> l \<noteq> to_literal (not l1)"
         hence "l = to_literal (not l1)" by simp
         hence "to_sl_formula l = (not l1)" by (simp add: \<open>l1 \<in> test_formulae\<close>)
-        hence "((ext_card_heap_superior_to n)::('var, 'k::finite) sl_formula) = not l1" using ndef by simp
-        also have "... = ((not (ext_card_heap_superior_to 0))::('var, 'k::finite) sl_formula)" using  l1_def by simp
-        finally have "((ext_card_heap_superior_to n)::('var, 'k::finite) sl_formula) = not (ext_card_heap_superior_to 0)" .
+        hence "((ext_card_heap_ge n)::('var, 'k::finite) sl_formula) = not l1" using ndef by simp
+        also have "... = ((not (ext_card_heap_ge 0))::('var, 'k::finite) sl_formula)" using  l1_def by simp
+        finally have "((ext_card_heap_ge n)::('var, 'k::finite) sl_formula) = not (ext_card_heap_ge 0)" .
         thus False 
         proof (cases "n = \<infinity>")
           case True
-          hence "ext_card_heap_superior_to n = sl_false" by simp
+          hence "ext_card_heap_ge n = sl_false" by simp
           thus ?thesis using  sl_formula.distinct
           proof -
             show ?thesis
-              by (metis \<open>ext_card_heap_superior_to (n::enat) = not (ext_card_heap_superior_to (0::enat))\<close> 
-                  \<open>ext_card_heap_superior_to (n::enat) = sl_false\<close> sl_formula.distinct(22))
+              by (metis \<open>ext_card_heap_ge (n::enat) = not (ext_card_heap_ge (0::enat))\<close> 
+                  \<open>ext_card_heap_ge (n::enat) = sl_false\<close> sl_formula.distinct(22))
           qed
         next
           case False
           show ?thesis
           proof (cases "n = 0")
             case True
-            hence "ext_card_heap_superior_to n = sl_true"
+            hence "ext_card_heap_ge n = sl_true"
               by (simp add: enat_defs(1)) 
             thus ?thesis
             proof -
               show ?thesis
-                by (metis \<open>ext_card_heap_superior_to n = not l1\<close> \<open>ext_card_heap_superior_to n = sl_true\<close> sl_formula.distinct(5))
+                by (metis \<open>ext_card_heap_ge n = not l1\<close> \<open>ext_card_heap_ge n = sl_true\<close> sl_formula.distinct(5))
             qed
           next
             case False
             hence "\<exists>m. n = Suc m" using \<open>n\<noteq> \<infinity>\<close> using list_decode.cases zero_enat_def by auto 
             from this obtain m where "n = Suc m" by auto
-            hence "ext_card_heap_superior_to (n::enat) = sl_conj (ext_card_heap_superior_to (m)) (not sl_emp)"
+            hence "ext_card_heap_ge (n::enat) = sl_conj (ext_card_heap_ge (m)) (not sl_emp)"
               by simp
             thus ?thesis
             proof -
               show ?thesis
-                by (metis (no_types) \<open>ext_card_heap_superior_to (n::enat) = 
-                  sl_conj (ext_card_heap_superior_to (enat (m::nat))) (not sl_emp)\<close> 
+                by (metis (no_types) \<open>ext_card_heap_ge (n::enat) = 
+                  sl_conj (ext_card_heap_ge (enat (m::nat))) (not sl_emp)\<close> 
                     \<open>to_sl_formula (l::('var, 'k) literal) = not (l1::('var, 'k) sl_formula)\<close> ndef 
                     sl_formula.distinct(57))
             qed
@@ -91,50 +91,50 @@ proof
       ultimately show "l = to_literal l1" by simp
     qed
     show "to_literal (not l1) \<in> x" by (simp add: l1_def x_def) 
-    show "\<exists>n. to_sl_formula (to_literal (not l1)) = not (ext_card_heap_superior_to n)"
+    show "\<exists>n. to_sl_formula (to_literal (not l1)) = not (ext_card_heap_ge n)"
     proof
-      show "to_sl_formula (to_literal (not l1)) = not (ext_card_heap_superior_to 0)" using \<open>l1\<in> test_formulae\<close>
+      show "to_sl_formula (to_literal (not l1)) = not (ext_card_heap_ge 0)" using \<open>l1\<in> test_formulae\<close>
         unfolding l1_def by simp     
     qed
-    show "\<And>l. l \<in> x \<and> (\<exists>n. to_sl_formula l = not (ext_card_heap_superior_to n)) \<Longrightarrow> l = to_literal (not l1)"
+    show "\<And>l. l \<in> x \<and> (\<exists>n. to_sl_formula l = not (ext_card_heap_ge n)) \<Longrightarrow> l = to_literal (not l1)"
     proof -
       fix l
-      assume lprop: "l \<in> x \<and> (\<exists>n. to_sl_formula l = not (ext_card_heap_superior_to n))"
-      hence "\<exists>n. to_sl_formula l = not (ext_card_heap_superior_to n)" by simp
-      from this obtain n where ndef: "to_sl_formula l = not (ext_card_heap_superior_to n)" by auto
+      assume lprop: "l \<in> x \<and> (\<exists>n. to_sl_formula l = not (ext_card_heap_ge n))"
+      hence "\<exists>n. to_sl_formula l = not (ext_card_heap_ge n)" by simp
+      from this obtain n where ndef: "to_sl_formula l = not (ext_card_heap_ge n)" by auto
       have "l = to_literal l1 \<or> l = to_literal (not l1)" using lprop unfolding x_def by simp
       moreover have "l\<noteq> to_literal (l1)"
       proof (rule ccontr)
         assume "\<not> l \<noteq> to_literal (l1)"
         hence "l = to_literal (l1)" by simp
         hence "to_sl_formula l = (l1)" by (simp add: \<open>l1 \<in> test_formulae\<close>)
-        hence "((not (ext_card_heap_superior_to n))::('var, 'k::finite) sl_formula) = l1" using ndef by simp
-        also have "... = (((ext_card_heap_superior_to 0))::('var, 'k::finite) sl_formula)" using  l1_def by simp
+        hence "((not (ext_card_heap_ge n))::('var, 'k::finite) sl_formula) = l1" using ndef by simp
+        also have "... = (((ext_card_heap_ge 0))::('var, 'k::finite) sl_formula)" using  l1_def by simp
         also have "... = (sl_true::('var, 'k::finite) sl_formula)" by (simp add: enat_defs)
-        finally have "((not (ext_card_heap_superior_to n))::('var, 'k::finite) sl_formula) = (sl_true)" .
+        finally have "((not (ext_card_heap_ge n))::('var, 'k::finite) sl_formula) = (sl_true)" .
         thus False 
         proof (cases "n = \<infinity>")
           case True
-          hence "ext_card_heap_superior_to n = sl_false" by simp
-          hence "not (ext_card_heap_superior_to n) = not sl_false" by simp
-          thus ?thesis using  sl_formula.distinct \<open>not (ext_card_heap_superior_to n) = sl_true\<close> by simp
+          hence "ext_card_heap_ge n = sl_false" by simp
+          hence "not (ext_card_heap_ge n) = not sl_false" by simp
+          thus ?thesis using  sl_formula.distinct \<open>not (ext_card_heap_ge n) = sl_true\<close> by simp
         next
           case False
           show ?thesis
           proof (cases "n = 0")
             case True
-            hence "ext_card_heap_superior_to n = sl_true"
+            hence "ext_card_heap_ge n = sl_true"
               by (simp add: enat_defs(1)) 
-            hence "not (ext_card_heap_superior_to n) = not sl_true" by simp
-            thus ?thesis using sl_formula.distinct \<open>not (ext_card_heap_superior_to n) = sl_true\<close> by simp
+            hence "not (ext_card_heap_ge n) = not sl_true" by simp
+            thus ?thesis using sl_formula.distinct \<open>not (ext_card_heap_ge n) = sl_true\<close> by simp
           next
             case False
             hence "\<exists>m. n = Suc m" using \<open>n\<noteq> \<infinity>\<close> using list_decode.cases zero_enat_def by auto 
             from this obtain m where "n = Suc m" by auto
-            hence "ext_card_heap_superior_to (n::enat) = sl_conj (ext_card_heap_superior_to (m)) (not sl_emp)"
+            hence "ext_card_heap_ge (n::enat) = sl_conj (ext_card_heap_ge (m)) (not sl_emp)"
               by simp
-            hence "not (ext_card_heap_superior_to n) = not (sl_conj (ext_card_heap_superior_to (m)) (not sl_emp))" by simp
-            thus ?thesis using sl_formula.distinct \<open>not (ext_card_heap_superior_to n) = sl_true\<close> by simp
+            hence "not (ext_card_heap_ge n) = not (sl_conj (ext_card_heap_ge (m)) (not sl_emp))" by simp
+            thus ?thesis using sl_formula.distinct \<open>not (ext_card_heap_ge n) = sl_true\<close> by simp
           qed
         qed
       qed
@@ -152,7 +152,15 @@ definition e_minterm::"('var, 'k::finite) minterm \<Rightarrow> ('var, 'k) sl_fo
 
 definition a_minterm::"('var, 'k::finite) minterm \<Rightarrow> ('var, 'k) sl_formula set"
   where "a_minterm M = {(Rep_literal l)|l. l \<in> (Rep_minterm M)} 
-                     \<inter> {alloc x|x. True}" 
+                     \<inter> {alloc x|x. True}"
+
+definition u_minterm::"('var, 'k::finite) minterm \<Rightarrow> ('var, 'k) sl_formula set"
+  where "u_minterm M = {(Rep_literal l)|l. l \<in> (Rep_minterm M)} 
+                     \<inter> ({ext_card_heap_ge n|n. True} \<union> {not (ext_card_heap_ge n)|n. True})"
+
+definition p_minterm::"('var, 'k::finite) minterm \<Rightarrow> ('var, 'k) sl_formula set"
+  where "p_minterm M = {(Rep_literal l)|l. l \<in> (Rep_minterm M)} 
+                     \<inter> ({points_to x y|x y. True} \<union> {not (points_to x y)|x y. True})"
 
 
 (* 3 lemmes:
@@ -161,6 +169,6 @@ definition a_minterm::"('var, 'k::finite) minterm \<Rightarrow> ('var, 'k) sl_fo
 - si a et b \<Rightarrow> mintern
 *)
 
-
+(* M = e_minter \<union> a_minterm \<union> u_minterm \<union> p_minterm *)
 
 end
